reloctablegen and relocbingen reconstruction

x86/RelocProgSemantics1.v
@@ -10,152 +10,14 @@ Require Import Events lib.Floats Memory Smallstep.
 Require Import Asm RelocProg RelocProgram Globalenvs.
 Require Import Locations Stacklayout Conventions.
 Require Import Linking Errors.
-Require RelocProgSemantics Reloctablesgen RelocProgSemanticsArchi1.
-Require Import LocalLib.
+Require Import RelocProgSemantics Reloctablesgen RelocProgSemanticsArchi RelocProgSemanticsArchi1.
+Require Import RelocProgGlobalenvs LocalLib.
 Import ListNotations.
 
 
 Section WITH_INSTR_SIZE.
   Variable instr_size : instruction -> Z.
 
-
-Definition rev_id_eliminate (symb: ident) (i:instruction) :=
-   match i with
-  | Pjmp_s id sg =>
-     (Pjmp_s symb sg)
-  | Pjmp_m (Addrmode rb ss (inr disp)) =>
-    let '(id, ptrofs) := disp in
-     (Pjmp_m (Addrmode rb ss (inr (symb,ptrofs))))
-  | Pcall_s id sg =>
-     (Pcall_s symb sg)
-  | Pmov_rs rd id =>
-     (Pmov_rs rd symb)
-  | Pmovl_rm rd (Addrmode rb ss (inr disp)) =>
-    let '(id, ptrofs) := disp in
-     (Pmovl_rm rd (Addrmode rb ss (inr (symb,ptrofs))))
-  | Pmovl_mr (Addrmode rb ss (inr disp)) rs =>
-    let '(id, ptrofs) := disp in
-     (Pmovl_mr (Addrmode rb ss (inr (symb, ptrofs))) rs)
-  | Pfldl_m (Addrmode rb ss (inr disp)) =>
-    let '(id, ptrofs) := disp in
-     (Pfldl_m (Addrmode rb ss (inr (symb, ptrofs))))
-  | Pfstpl_m (Addrmode rb ss (inr disp)) =>
-    let '(id, ptrofs) := disp in
-     (Pfstpl_m (Addrmode rb ss (inr (symb, ptrofs))))
-  | Pflds_m (Addrmode rb ss (inr disp)) =>
-    let '(id, ptrofs) := disp in
-     (Pflds_m (Addrmode rb ss (inr (symb, ptrofs))))
-  | Pfstps_m (Addrmode rb ss (inr disp)) =>
-    let '(id, ptrofs) := disp in
-     (Pfstps_m (Addrmode rb ss (inr (symb, ptrofs))))
-  | Pmovsd_fm rd (Addrmode rb ss (inr disp)) =>
-    let '(id, ptrofs) := disp in
-     (Pmovsd_fm rd (Addrmode rb ss (inr (symb, ptrofs))))
-  | Pmovsd_mf (Addrmode rb ss (inr disp)) rs =>
-    let '(id, ptrofs) := disp in
-    (Pmovsd_mf (Addrmode rb ss (inr (symb, ptrofs))) rs)
-  | Pmovsd_fm_a rd (Addrmode rb ss (inr disp)) =>
-    let '(id, ptrofs) := disp in
-    (Pmovsd_fm rd (Addrmode rb ss (inr (symb, ptrofs))))
-  | Pmovsd_mf_a (Addrmode rb ss (inr disp)) rs =>
-    let '(id, ptrofs) := disp in
-     (Pmovsd_mf (Addrmode rb ss (inr (symb, ptrofs))) rs)  
-  | Pmovss_fm rd (Addrmode rb ss (inr disp)) =>
-    let '(id, ptrofs) := disp in
-     (Pmovss_fm rd (Addrmode rb ss (inr (symb, ptrofs))))
-  | Pmovss_mf (Addrmode rb ss (inr disp)) rs =>
-    let '(id, ptrofs) := disp in
-     (Pmovss_mf (Addrmode rb ss (inr (symb, ptrofs))) rs)
-  | Pxorpd_fm rd (Addrmode rb ss (inr disp)) =>
-    let '(id, ptrofs) := disp in
-     (Pxorpd_fm rd (Addrmode rb ss (inr (symb, ptrofs))))
-  | Pxorps_fm rd (Addrmode rb ss (inr disp)) =>
-    let '(id, ptrofs) := disp in
-     (Pxorps_fm rd (Addrmode rb ss (inr (symb, ptrofs))))
-  | Pandpd_fm rd (Addrmode rb ss (inr disp)) =>
-    let '(id, ptrofs) := disp in
-     (Pandpd_fm rd (Addrmode rb ss (inr (symb, ptrofs))))
-  | Pandps_fm rd (Addrmode rb ss (inr disp)) =>
-    let '(id, ptrofs) := disp in
-     (Pandps_fm rd (Addrmode rb ss (inr (symb, ptrofs))))
-  (** Moves with conversion *)
-  | Pmovb_mr (Addrmode rb ss (inr disp)) rs =>
-    let '(id, ptrofs) := disp in
-     (Pmovb_mr (Addrmode rb ss (inr (symb, ptrofs))) rs)
-  | Pmovb_rm rd (Addrmode rb ss (inr disp)) =>
-    let '(id, ptrofs) := disp in
-     (Pmovb_rm rd (Addrmode rb ss (inr (symb, ptrofs))))
-  | Pmovw_mr (Addrmode rb ss (inr disp)) rs =>
-    let '(id, ptrofs) := disp in
-     (Pmovw_mr (Addrmode rb ss (inr (symb, ptrofs))) rs)
-  | Pmovw_rm rd (Addrmode rb ss (inr disp)) =>
-    let '(id, ptrofs) := disp in
-     (Pmovw_rm rd (Addrmode rb ss (inr (symb, ptrofs))))
-  | Pmovzb_rm rd (Addrmode rb ss (inr disp)) =>
-    let '(id, ptrofs) := disp in
-     (Pmovzb_rm rd (Addrmode rb ss (inr (symb, ptrofs))))
-  | Pmovsb_rm rd (Addrmode rb ss (inr disp)) =>
-    let '(id, ptrofs) := disp in
-     (Pmovsb_rm rd (Addrmode rb ss (inr (symb, ptrofs))))
-  | Pmovzw_rm rd (Addrmode rb ss (inr disp)) =>
-    let '(id, ptrofs) := disp in
-     (Pmovzw_rm rd (Addrmode rb ss (inr (symb, ptrofs))))
-  | Pmovsw_rm rd (Addrmode rb ss (inr disp)) =>
-    let '(id, ptrofs) := disp in
-     (Pmovsw_rm rd (Addrmode rb ss (inr (symb, ptrofs))))
-  | Pmovsq_rm rd (Addrmode rb ss (inr disp)) =>
-    let '(id, ptrofs) := disp in
-     (Pmovsq_rm rd (Addrmode rb ss (inr (symb, ptrofs))))
-  | Pmovsq_mr (Addrmode rb ss (inr disp)) rs =>
-    let '(id, ptrofs) := disp in
-     (Pmovsq_mr (Addrmode rb ss (inr (symb, ptrofs))) rs)
-  (** Integer arithmetic *)
-  | Pleal rd (Addrmode rb ss (inr disp))  =>
-    let '(id, ptrofs) := disp in
-     (Pleal rd (Addrmode rb ss (inr (symb, ptrofs))))
-  (** Saving and restoring registers *)
-  | Pmov_rm_a rd (Addrmode rb ss (inr disp)) =>  (**r like [Pmov_rm], using [Many64] chunk *)
-    let '(id, ptrofs) := disp in
-     (Pmov_rm_a rd (Addrmode rb ss (inr (symb, ptrofs))))
-  | Pmov_mr_a (Addrmode rb ss (inr disp)) rs =>   (**r like [Pmov_mr], using [Many64] chunk *)
-    let '(id, ptrofs) := disp in
-    (Pmov_mr_a (Addrmode rb ss (inr (symb, ptrofs))) rs)
-  | Paddq_rm rd (Addrmode rb ss (inr disp))  =>
-    let '(id, ptrofs) := disp in
-    (Paddq_rm rd (Addrmode rb ss (inr (symb, ptrofs))))
-  | Psubq_rm rd (Addrmode rb ss (inr disp))  =>
-    let '(id, ptrofs) := disp in
-    (Psubq_rm rd (Addrmode rb ss (inr (symb, ptrofs))))
-  | Pimulq_rm rd (Addrmode rb ss (inr disp))  =>
-    let '(id, ptrofs) := disp in
-    (Pimulq_rm rd (Addrmode rb ss (inr (symb, ptrofs))))
-  | Pandq_rm rd (Addrmode rb ss (inr disp))  =>
-    let '(id, ptrofs) := disp in
-    (Pandq_rm rd (Addrmode rb ss (inr (symb, ptrofs))))
-  | Porq_rm rd (Addrmode rb ss (inr disp))  =>
-    let '(id, ptrofs) := disp in
-    (Porq_rm rd (Addrmode rb ss (inr (symb, ptrofs))))
-  | Pxorq_rm rd (Addrmode rb ss (inr disp))  =>
-    let '(id, ptrofs) := disp in
-    (Pxorq_rm rd (Addrmode rb ss (inr (symb, ptrofs))))
-  | Pcmpq_rm rd (Addrmode rb ss (inr disp))  =>
-    let '(id, ptrofs) := disp in
-    (Pcmpq_rm rd (Addrmode rb ss (inr (symb, ptrofs))))
-  | Ptestq_rm rd (Addrmode rb ss (inr disp))  =>
-    let '(id, ptrofs) := disp in
-    (Ptestq_rm rd (Addrmode rb ss (inr (symb, ptrofs))))
-  | Pmovq_rm rd (Addrmode rb ss (inr disp))  =>
-    let '(id, ptrofs) := disp in
-    (Pmovq_rm rd (Addrmode rb ss (inr (symb, ptrofs))))
-  | Pmovq_mr (Addrmode rb ss (inr disp)) rs =>
-    let '(id, ptrofs) := disp in
-    (Pmovq_mr (Addrmode rb ss (inr (symb, ptrofs))) rs)
-  | Pleaq rd (Addrmode rb ss (inr disp))  =>
-    let '(id, ptrofs) := disp in
-     (Pleaq rd (Addrmode rb ss (inr (symb, ptrofs))))
-  | _ =>
-     i
-    end.
 
 Definition rev_acc_code (r:code*Z*reloctable) i :=
   let '(c,ofs,reloctbl) := r in
@@ -208,7 +70,7 @@ Definition semantics (p:program) (rs:regset) :=
                 (initial_state p rs)
                 (RelocProgSemantics.final_state)
                 (globalenv p)
-                (RelocProgSemantics.Genv.genv_senv (RelocProgSemantics.globalenv instr_size p)).
+                (Genv.genv_senv (RelocProgSemantics.globalenv instr_size p)).
 
 Lemma semantics_determinate: forall p rs, determinate (semantics p rs).
 Proof.
@@ -226,7 +88,7 @@ Proof.
     + split. constructor. auto.
     + discriminate.
     + discriminate.
-    + assert (vargs0 = vargs) by (eapply RelocProgSemantics.eval_builtin_args_determ; eauto).     
+    + assert (vargs0 = vargs) by (eapply RelocProgSemanticsArchi.eval_builtin_args_determ; eauto).     
       subst vargs0.      
       exploit external_call_determ. eexact H5. eexact H11. intros [A B].      
       split. auto. intros. destruct B; auto. subst. auto.
