x86/RelocBingenproofArchi.v
@@ -1,0 +1,292 @@
+Require Import Coqlib Maps AST lib.Integers Values.
+Require Import Events lib.Floats Memory Smallstep.
+Require Import Asm RelocProg RelocProgramBytes.
+Require Import Stacklayout Conventions.
+Require Import Linking RelocProgLinking Errors.
+Require Import EncDecRet RelocBingen RelocBinDecode.
+Require Import RelocProgSemantics RelocProgSemantics1.
+Require Import TranslateInstr RelocProgSemantics2.
+Require Import RelocProgSemantics RelocProgSemantics1 RelocProgSemanticsArchi1.
+Require Import RelocProgSemanticsArchi RelocProgGlobalenvs.
+
+Import ListNotations.
+Local Open Scope error_monad_scope.
+
+Lemma PTree_map_elements: forall A B (f:positive -> A -> B) m,
+    let R := (fun p a b => f p a = b) in
+    list_forall2
+      (fun (i_x : positive * A) (i_y : positive * B) =>
+         fst i_x = fst i_y /\ R (fst i_x) (snd i_x) (snd i_y))
+      (PTree.elements m) (PTree.elements (PTree.map f m)).
+Proof.
+  intros.
+  apply PTree.elements_canonical_order1;intros.
+  - unfold R in *.
+    rewrite PTree.gmap.
+    rewrite H. simpl. exists (f i x). auto.
+  - unfold R in *.
+    rewrite PTree.gmap in H.
+    unfold option_map in *. destr_in H.
+    exists a. inv H. auto.
+Qed.
+
+Section WITH_INSTR_SIZE.
+  Variable instr_size: instruction -> Z.
+  Variable Instr_size: list Instruction -> Z.
+(* used in gen_instr_map_refl *)
+Lemma rev_id_eliminate_instr_eq: forall i1 i2 id,
+    instr_eq i1 i2 ->
+    instr_eq (rev_id_eliminate id i1) (rev_id_eliminate id i2).
+Proof.
+  intros.
+  unfold instr_eq in H. destruct H.
+    (* i = i1 *)
+  subst. left. auto.
+
+  (* i is not well defined *)
+  destruct i1;try inv H;destr_in H;subst.
+  1-10: try (try destruct H;subst;simpl;unfold instr_eq;auto).
+
+  1-6 :
+    try (try destr_in H;destruct H;subst;
+         simpl;do 2 destr;
+         unfold instr_eq; try rewrite Heqb; auto;
+         
+         destruct p; unfold instr_eq; try rewrite Heqb; auto).
+ 
+  destruct H. subst. simpl. do 2 destr. unfold instr_eq. auto.
+  destruct p; unfold instr_eq; auto.
+  destruct H. subst. simpl. do 2 destr. unfold instr_eq. auto.
+  destruct p; unfold instr_eq; auto.
+
+  simpl. unfold instr_eq. right. auto.
+  
+Qed.
+
+Lemma eval_addrmode_match_ge: forall ge1 ge2 a rs (MATCHGE: forall i ofs, RelocProgGlobalenvs.Genv.symbol_address ge1 i ofs = RelocProgGlobalenvs.Genv.symbol_address ge2 i ofs),
+    RelocProgSemanticsArchi.eval_addrmode ge1 a rs = eval_addrmode ge2 a rs.
+Proof.
+  unfold eval_addrmode. destruct Archi.ptr64;intros.
+  - unfold eval_addrmode64.
+    destruct a. f_equal.
+    f_equal. destr.
+    destruct p. eauto.
+  - unfold eval_addrmode32.
+    destruct a. f_equal.
+    f_equal. destr.
+    destruct p. eauto.
+Qed.
+
+Lemma exec_load_match_ge: forall sz ge1 ge2 chunk m a rs rd (MATCHGE: forall i ofs, RelocProgGlobalenvs.Genv.symbol_address ge1 i ofs = RelocProgGlobalenvs.Genv.symbol_address ge2 i ofs) ,
+          exec_load sz ge1 chunk m a rs rd = exec_load sz ge2 chunk m a rs rd.
+Proof.
+  unfold exec_load.
+  intros. erewrite eval_addrmode_match_ge.
+  eauto. auto.
+Qed.
+
+Lemma exec_store_match_ge: forall sz ge1 ge2 chunk m a rs rd l (MATCHGE: forall i ofs, RelocProgGlobalenvs.Genv.symbol_address ge1 i ofs = RelocProgGlobalenvs.Genv.symbol_address ge2 i ofs) ,
+          exec_store sz ge1 chunk m a rs rd l = exec_store sz ge2 chunk m a rs rd l.
+Proof.
+  unfold exec_store.
+  intros. erewrite eval_addrmode_match_ge.
+  eauto. auto.
+Qed.
+
+(* ad-hoc *)
+Section PRESERVATION. 
+(** Transformation *)
+  Variable prog: RelocProgram.program.
+  Variable tprog: program.
+  
+  
+  Let ge := RelocProgSemantics1.globalenv instr_size prog.
+  Let tge := RelocProgSemantics2.globalenv instr_size Instr_size tprog.
+  
+  Hypothesis symbol_address_pres: forall id ofs,
+    RelocProgGlobalenvs.Genv.symbol_address ge id ofs =
+    RelocProgGlobalenvs.Genv.symbol_address tge id ofs.
+  Hypothesis find_instr_refl: forall b ofs i,
+    Genv.genv_instrs ge b ofs = Some i ->
+    exists i1, Genv.genv_instrs tge b ofs = Some i1
+          /\ instr_eq i i1.
+  Hypothesis find_ext_funct_refl: forall v,
+    Genv.find_ext_funct ge v = Genv.find_ext_funct tge v.
+  Hypothesis instr_eq_size: forall i1 i2, instr_eq i1 i2 -> instr_size i1 = instr_size i2.
+  Hypothesis rev_transl_code_in: forall i c r,
+    In i (rev_transl_code instr_size r c) ->
+    exists i', In i' c /\ ((exists id, rev_id_eliminate id i' = i) \/ i = i').
+  Hypothesis transl_instr_in_code: forall c i id,
+    prog.(prog_sectable) ! id = Some (sec_text c) ->
+    In i c ->
+    exists i' e, translate_instr e i = OK i'.
+  Hypothesis senv_refl:
+    (Genv.genv_senv ge) = (Genv.genv_senv tge).
+
+  
+Lemma exec_instr_refl: forall i rs m,
+    exec_instr instr_size ge i rs m = exec_instr instr_size tge i rs m.
+Proof.
+  destruct i;simpl;auto;intros.
+  1-27: try (erewrite symbol_address_pres;eauto).
+  1-24: try (erewrite exec_load_match_ge;eauto;eapply symbol_address_pres;eauto).
+  1-12: try (erewrite exec_store_match_ge;eauto;eapply symbol_address_pres;eauto).
+  do 3 f_equal.
+  unfold eval_addrmode32.
+  destruct a. f_equal.
+  f_equal. destr.
+  destruct p. eapply symbol_address_pres;eauto.
+  do 3 f_equal.
+  unfold eval_addrmode64.
+  destruct a. f_equal.
+  f_equal. destr.
+  destruct p. eapply symbol_address_pres;eauto.
+Qed.
+
+
+Lemma eval_addrmode_refl: forall a rs,
+    eval_addrmode ge a rs = eval_addrmode tge a rs.
+Proof.
+  intros.
+  erewrite eval_addrmode_match_ge. eauto.
+  apply symbol_address_pres.
+Qed. 
+
+  
+Lemma step_simulation: forall st1 st2 t,
+    step instr_size ge st1 t st2 ->
+    step instr_size tge st1 t st2.
+Proof.
+  intros st1 st2 t STEP.
+  inv STEP.
+  - unfold Genv.find_instr in H1.
+    exploit find_instr_refl;eauto.
+    intros (i1 & FIND & MATCHINSTR).
+    eapply exec_step_internal;eauto.
+    erewrite <- find_ext_funct_refl;eauto.
+    exploit instr_eq_size;eauto. intros SIZE.
+    unfold instr_eq in MATCHINSTR. destruct MATCHINSTR.
+    (* i = i1 *)
+    subst. rewrite <- exec_instr_refl. auto.
+
+  (* i is not well defined *)
+    destruct i;try inv H3;simpl in H2;destr_in H3.
+    (* Pmovzl_rr *)
+    + inv H3. simpl.
+      admit.
+    (* Pmovls_rr *)
+    + subst. simpl.
+      admit.
+    (* Pxorl_rr *)
+    + destruct H3;subst.
+      simpl.
+      admit.
+    (* Pxorq_rr r1 <> r2 *)
+    + destruct H3;subst.
+      destruct H4;subst.
+      simpl. auto.
+    (* Pxorq_rr *)
+    + destruct H3;subst.
+      simpl.
+      admit.
+    (* Pxorq_rr r1 <> r2 *)
+    + destruct H3;subst.
+      destruct H4;subst.
+      simpl. auto.
+
+    (* Pjmp_s *)
+    + subst. simpl.
+      rewrite <- symbol_address_pres.
+      auto.
+    (* Pjmp_r *)
+    + subst. simpl. auto.
+    (* Pcall_s *)
+    + subst. simpl.
+      rewrite SIZE in *.
+      destr_in H2.
+      (* rewrite <- symbol_address_pres. *)
+      (* auto. *)
+    (* Pcall_r *)
+    + subst. simpl.
+      rewrite SIZE in *.
+      destr_in H2.
+      
+    (* Pmov_rm_a 32 *)
+    + destr_in H3.
+      destruct H3;subst.
+      simpl.
+      unfold exec_load in *.
+      unfold Mem.loadv in *.
+      rewrite <- eval_addrmode_refl.
+      destr_in H2.
+      destr_in Heqo.
+      Transparent Mem.load. 
+      assert (Mem.load  Many32 m b0
+                        (Ptrofs.unsigned i) = Mem.load Mint32 m b0 (Ptrofs.unsigned i)).
+      { unfold Mem.load.
+        unfold Mem.valid_access_dec.
+        cbn [size_chunk]. cbn [align_chunk].
+        destruct (Mem.range_perm_dec m b0 (Ptrofs.unsigned i)
+                                     (Ptrofs.unsigned i + 4) Cur Readable).
+        destruct (Zdivide_dec 4 (Ptrofs.unsigned i)).
+        unfold size_chunk_nat. cbn [size_chunk].
+        f_equal. unfold decode_val.
+        rewrite Heqb0.
+        admit. auto. auto. }
+      rewrite <- H3. rewrite Heqo.
+      admit.
+
+    (* Pmov_rm_a 64 *)
+    + admit.
+    (* Pmov_mr_a 32 *)
+    + admit.
+    (* Pmov_mr_a 64 *)
+    + admit.
+    (* Pmovsd_fm_a *)
+    + admit.
+    (* Pmovsd_mf_a *)
+    + admit.
+    + simpl. rewrite SIZE in *.
+      auto.
+
+  (* Pbuiltin instr impossible *)
+  - unfold Genv.find_instr in H1.
+    simpl in H1. apply gen_code_map_inv in H1.
+    destruct H1 as (id & c & P1 & P2 & P3).
+    generalize (PTree_map_elements _ (RelocProg.section instruction init_data) (rev_section instr_size (prog_reloctables prog)) (prog_sectable prog)). simpl.
+    intros F.
+    apply PTree.elements_correct in P2.
+    exploit list_forall2_in_right;eauto.
+    simpl.
+    intros (x1 & In1 & ? &REV1).
+    subst. destruct x1. apply PTree.elements_complete in In1.
+    simpl in REV1.
+    destruct s.  2-3:  simpl in REV1; congruence.
+    simpl in REV1. destr_in REV1.
+    + inv REV1. apply rev_transl_code_in in P3.
+      destruct P3 as (i' & In' & P3').
+      assert (i' = Pbuiltin ef args res).
+      { destruct P3'.
+        destruct H1 as (id & P3').
+        destruct i';simpl in P3';repeat destr_in P3';try congruence.
+        subst. auto. }
+      subst.
+      
+      eapply transl_instr_in_code in In1;eauto.
+      simpl in In1. destruct In1 as (? & ? & ?).
+      inv H1.
+      
+    + inv REV1.
+      eapply transl_instr_in_code in In1;eauto.
+      destruct In1 as (? & ? & ?).
+      inv H1.
+      
+  - 
+    rewrite find_ext_funct_refl in H0.
+    eapply exec_step_external;eauto.
+    rewrite <- senv_refl. auto.
+Admitted.
+
+End PRESERVATION.
+
+End WITH_INSTR_SIZE.
