x86/ReloctablesgenproofArchi.v
@@ -1,0 +1,160 @@
+Require Import Coqlib Errors Maps.
+Require Import Integers Floats AST RelocProgLinking Linking.
+Require Import Op Locations Mach Conventions Asm RealAsm.
+Require Import Reloctablesgen ReloctablesgenArchi.
+Require Import RelocProg RelocProgram RelocProgSemantics RelocProgSemantics1.
+Require Import RelocProgSemanticsArchi1.
+Require Import LocalLib AsmInject.
+Import ListNotations.
+Require AsmFacts.
+
+Section WITH_INSTR_SIZE.
+
+Variable instr_size : instruction -> Z.
+Hypothesis instr_size_bound : forall i, 0 < instr_size i <= Ptrofs.max_unsigned.
+Hypothesis instr_reloc_bound : forall i ofs, instr_reloc_offset i = OK ofs -> 0 < ofs < instr_size i.
+Hypothesis id_eliminate_size_unchanged:forall i, instr_size i = instr_size (id_eliminate i).
+
+Lemma lt_add_range:forall a b c,
+    0 < b < c -> a < a + b < a + c.
+Proof. 
+  intros. lia.
+Qed.
+
+Lemma code_id_eliminate_size_unchanged:forall c,
+    code_size instr_size (transl_code' c) = code_size instr_size c.
+Proof.
+  intros. unfold transl_code'.
+  induction c;simpl;auto.
+  rewrite IHc. rewrite <- id_eliminate_size_unchanged.
+  auto.
+Qed.
+
+Lemma transl_instr_range: forall symbtbl ofs i e,
+    transl_instr instr_size symbtbl ofs i = OK (Some e) ->
+    ofs < e.(reloc_offset) < ofs + instr_size i.
+  intros symbtbl ofs i e.
+  generalize (instr_size_bound i). intros A.  
+  unfold transl_instr.
+  destruct i;simpl;intros;inv H.
+
+  (* only solve Pmov_rs *)  
+  monadInv H1.
+  unfold compute_instr_abs_relocentry in *. monadInv EQ.
+  destr_match_in EQ1;inv EQ1;simpl;eapply lt_add_range; auto.
+            
+  1-42: try (destruct a;destruct const;try destruct p;inv H1).
+  1-42: try (monadInv H0;
+             destruct Archi.ptr64;
+        unfold compute_instr_abs_relocentry in *;
+       unfold compute_instr_disp_relocentry in *;
+       unfold compute_instr_rel_relocentry in *;
+       repeat (monadInv EQ));
+    try (destr_match_in EQ1;inv EQ1;simpl).
+
+  1-79: try (eapply lt_add_range; auto).
+
+  1-42 : try(destr_match_in EQ2;inv EQ2;simpl;
+             eapply lt_add_range; auto).
+  
+  (* Pjmp_s *)
+  destruct Archi.ptr64. monadInv H1.
+  unfold compute_instr_rel_relocentry in *.
+  monadInv EQ.
+  destr_match_in EQ2;inv EQ2;simpl;eapply lt_add_range; auto.
+  inv H1. simpl. eapply lt_add_range; auto.
+  (* Pjmp_m *)
+  destruct base. monadInv H0.
+  unfold compute_instr_abs_relocentry in *.
+  monadInv EQ. 
+  destr_match_in EQ1;inv EQ1;simpl;eapply lt_add_range; auto.
+  destruct ofs0. monadInv H0.
+  unfold compute_instr_abs_relocentry in *.
+  monadInv EQ.
+  destr_match_in EQ1;inv EQ1;simpl;eapply lt_add_range; auto.
+  try (monadInv H0;
+             destruct Archi.ptr64;
+        unfold compute_instr_abs_relocentry in *;
+       unfold compute_instr_disp_relocentry in *;
+       unfold compute_instr_rel_relocentry in *;
+       repeat (monadInv EQ));
+    try (destr_match_in EQ1;inv EQ1;simpl).
+  destr_match_in EQ2;inv EQ2;simpl;eapply lt_add_range; auto.
+  eapply lt_add_range; auto.
+  (* call_s *)
+  destruct Archi.ptr64.
+  monadInv H1. unfold compute_instr_rel_relocentry in *. repeat (monadInv EQ). destr_match_in EQ2. inv EQ2.
+  simpl. 
+  eapply lt_add_range; auto. inv EQ2.
+  inv H1.   simpl. 
+  eapply lt_add_range; auto.
+  (* Pbuiltin *)
+  destr_match_in H1.
+  inv H1. inv H1.
+  (* Pmovw_rm *)
+  destruct ad;destruct const;try destruct p;inv H1.
+  monadInv H0. destruct Archi.ptr64.
+  unfold compute_instr_rel_relocentry in *.
+  monadInv EQ. destr_match_in EQ2. inv EQ2. simpl.
+  eapply lt_add_range; auto.
+  inv EQ2.
+  unfold compute_instr_abs_relocentry in *.
+  monadInv EQ. destr_match_in EQ1. inv EQ1. simpl.
+  eapply lt_add_range; auto. inv EQ1.
+Qed.
+
+Lemma transl_instr_consistency: forall i symbtbl ofs e,
+    transl_instr instr_size symbtbl ofs i = OK (Some e) ->
+    rev_id_eliminate (reloc_symb e) (id_eliminate i) = i.
+Proof.
+  intros i symbtbl ofs e.
+  destruct i;simpl;auto;
+    unfold transl_instr;simpl;intros H;repeat (monadInv H);
+      unfold compute_instr_disp_relocentry in *;
+      destruct Archi.ptr64;
+      unfold compute_instr_abs_relocentry in *;      
+    unfold compute_instr_rel_relocentry in *;
+    repeat (monadInv EQ);
+    try (destruct (symbtbl ! id);inv EQ1;simpl;auto); (* no addrmode finish *)
+    try (destruct a;destruct const;try destruct p;try congruence);
+  try (monadInv H;
+       unfold compute_instr_abs_relocentry in *;
+       unfold compute_instr_disp_relocentry in *;
+       unfold compute_instr_rel_relocentry in *;
+       repeat (monadInv EQ);
+       try (destr_in EQ1;inv EQ1;simpl;auto)).
+
+  1-45: try (destruct PTree.get;inv EQ2;simpl;auto).
+  1-4 : simpl;auto.
+  (* Pjmp_m *)
+  destruct base. monadInv H.
+  monadInv EQ. destruct PTree.get;inv EQ1;simpl;auto.
+  destruct ofs0. monadInv H.
+  monadInv EQ. destruct PTree.get;inv EQ1;simpl;auto.
+  monadInv H. monadInv EQ.
+  destruct PTree.get;inv EQ2;simpl;auto.
+  destruct base. monadInv H.
+  monadInv EQ. destruct PTree.get;inv EQ1;simpl;auto.
+  destruct ofs0. monadInv H.
+  monadInv EQ. destruct PTree.get;inv EQ1;simpl;auto.
+  monadInv H. monadInv EQ.
+  destruct PTree.get;inv EQ1;simpl;auto.
+
+  (* Pmovw *)
+  destruct ad;destruct const;try destruct p;try congruence.
+  monadInv H. monadInv EQ. destruct PTree.get;inv EQ2;simpl;auto.
+  destruct ad;destruct const;try destruct p;try congruence.
+  monadInv H. monadInv EQ. destruct PTree.get;inv EQ1;simpl;auto.
+  
+Qed.
+
+Lemma id_eliminate_unchanged:forall i symbtbl ofs,
+    transl_instr instr_size symbtbl ofs i = OK None ->
+    id_eliminate i = i.
+Proof.
+  intros i symbtl ofs.
+  destruct i;simpl;auto;
+  unfold transl_instr;simpl;intros;repeat (monadInv H);repeat (destr_in H);repeat monadInv H1.
+Qed.
+
+End WITH_INSTR_SIZE.
